feat: start inferLvl experiment

GroupoidModel/Russell_PER_MS/Basic.lean
@@ -11,11 +11,11 @@ inductive Expr where
   /-- De Bruijn index. -/
   | bvar (i : Nat)
   /-- Dependent product. -/
-  | pi (l l' : Nat) (A B : Expr)
+  | pi (A B : Expr)
   /-- Lambda. -/
-  | lam (l l' : Nat) (ty body : Expr)
+  | lam (ty body : Expr)
   /-- Application at the specified output type. -/
-  | app (l l' : Nat) (B fn arg : Expr)
+  | app (B fn arg : Expr)
   /-- (Russell) type universe. -/
   | univ (l : Nat)
   /-- Type from a code. -/
@@ -23,3 +23,40 @@ inductive Expr where
   /-- Code from a type. -/
   | code (A : Expr) : Expr
   deriving Repr
+
+@[reducible]
+def Expr.size : Expr → Nat
+  | bvar _ => 1
+  | pi A B => A.size + B.size + 1
+  | lam A e => A.size + e.size + 1
+  | app B fn arg => B.size + fn.size + arg.size + 1
+  | univ _ => 1
+  | el a => a.size + 1
+  | code A => A.size + 1
+
+@[simp]
+theorem Expr.size_pos (e : Expr) : 0 < e.size := by
+  induction e <;> { dsimp [size]; omega }
+
+@[simp]
+theorem Expr.size_lt_pi_size (A B : Expr) : A.size < (pi A B).size := by
+  dsimp [size]; omega
+
+@[simp]
+theorem Expr.size_lt_app_size (B fn arg : Expr) : B.size < (app B fn arg).size := by
+  dsimp [size]; omega
+
+/-- `inferLvl Γ e` is such that
+- if `Γ ⊢[l] e : A`, then `l = inferLvl Γ e`; and
+- if `Γ ⊢[l] e` then `l = inferLvl Γ e`. -/
+def Expr.inferLvl : List Expr → Expr → Nat
+  | [],      bvar _       => 1337
+  | A :: As, bvar 0       => inferLvl As A
+  | _ :: As, bvar (i + 1) => inferLvl As (bvar i)
+  | Γ,       pi A B       => max (inferLvl Γ A) (inferLvl (A :: Γ) B)
+  | Γ,       lam A e      => max (inferLvl Γ A) (inferLvl (A :: Γ) e)
+  | Γ,       app B _ _    => inferLvl Γ B
+  | _,       univ l       => l + 1
+  | Γ,       el a         => inferLvl Γ a - 1
+  | Γ,       code a       => inferLvl Γ a + 1
+termination_by Γ e => (e :: Γ).map Expr.size |>.sum
