GroupoidModel/Russell_PER_MS/Typing.lean
@@ -22,7 +22,10 @@ macro_rules
 
 end Notation
 
-/-- `Lookup Γ i A` implies that `Γ ⊢ .bvar i : A`. -/
+/-- `Lookup Γ i A` means that `A` appears on the `i`-th position in `Γ`.
+
+Note this is _not_ closed under context or type defeq. -/
+-- Q: does L4L have another version of this that is closed?
 inductive Lookup : List Expr → Nat → Expr → Prop where
   | zero {Γ A} : Lookup (A::Γ) 0 A.lift
   | succ {Γ i A} : Lookup Γ i A → Lookup (A::Γ) (i+1) A.lift
@@ -44,7 +47,7 @@ inductive EqTp : List Expr → Nat → Expr → Expr → Prop
   | cong_pi {Γ A A' B B' l l'} :
     Γ ⊢[l] A ≡ A'→
     A :: Γ ⊢[l'] B ≡ B' →
-    Γ ⊢[max l l'] .pi l l' A B ≡ .pi l l' A' B'
+    Γ ⊢[max l l'] .pi A B ≡ .pi A' B'
 
   | cong_univ (Γ l) :
     l < univMax →
@@ -55,7 +58,7 @@ inductive EqTp : List Expr → Nat → Expr → Expr → Prop
     Γ ⊢[l] .el A ≡ .el A'
 
   -- Substitution
-  | inst {Γ A B B' t u l l'} :
+  | inst_tp {Γ A B B' t u l l'} :
     A :: Γ ⊢[l] B ≡ B' →
     Γ ⊢[l'] t ≡ u : A →
     Γ ⊢[l] B.inst t ≡ B.inst u
@@ -82,13 +85,13 @@ inductive EqTm : List Expr → Nat → Expr → Expr → Expr → Prop
   | cong_lam {Γ A A' B t t' l l'} :
     Γ ⊢[l] A ≡ A' →
     A :: Γ ⊢[l'] t ≡ t' : B →
-    Γ ⊢[max l l'] .lam l l' A t ≡ .lam l l' A' t' : .pi l l' A B
+    Γ ⊢[max l l'] .lam A t ≡ .lam A' t' : .pi A B
 
   | cong_app {Γ A B B' f f' a a' l l'} :
     A :: Γ ⊢[l'] B ≡ B' →
-    Γ ⊢[max l l'] f ≡ f' : .pi l l' A B →
+    Γ ⊢[max l l'] f ≡ f' : .pi A B →
     Γ ⊢[l] a ≡ a' : A →
-    Γ ⊢[l'] .app l l' B f a ≡ .app l l' B' f' a' : B.inst a
+    Γ ⊢[l'] .app B f a ≡ .app B' f' a' : B.inst a
 
   | cong_code {Γ A A' l} :
     l < univMax →
@@ -96,7 +99,7 @@ inductive EqTm : List Expr → Nat → Expr → Expr → Expr → Prop
     Γ ⊢[l+1] .code A ≡ .code A' : .univ l
 
   -- Substitution
-  | inst {Γ A B t u a b l l'} :
+  | inst_tm {Γ A B t u a b l l'} :
     A :: Γ ⊢[l] t ≡ u : B →
     Γ ⊢[l'] a ≡ b : A →
     Γ ⊢[l] t.inst a ≡ u.inst b : B.inst a
@@ -107,12 +110,12 @@ inductive EqTm : List Expr → Nat → Expr → Expr → Expr → Prop
   | app_lam {Γ A B t u l l'} :
     A :: Γ ⊢[l'] t : B →
     Γ ⊢[l] u : A →
-    Γ ⊢[l'] .app l l' B (.lam l l' A t) u ≡ t.inst u : B.inst u
+    Γ ⊢[l'] .app B (.lam A t) u ≡ t.inst u : B.inst u
 
   -- Expansions
   | eta {Γ A B t l l'} :
-    Γ ⊢[max l l'] t : .pi l l' A B →
-    Γ ⊢[max l l'] t ≡ .lam l l' A (.app l l' B t.lift (.bvar 0)) : .pi l l' A B
+    Γ ⊢[max l l'] t : .pi A B →
+    Γ ⊢[max l l'] t ≡ .lam A (.app B t.lift (.bvar 0)) : .pi A B
 
   -- Conversion
   | conv {Γ A A' t t' l} :
